Adaptive_State_Counting/ASC/ASC_Example.thy
@@ -427,35 +427,42 @@ lemma precondition_not_vacuous :
            (PM::(nat,nat,nat\<times>nat) FSM)
            (V::(nat list set)) 
            (\<Omega>::(nat,nat) ATC set)
-           (m :: nat) . OFSM M1 \<and> OFSM M2 \<and> asc_fault_domain M2 M1 m \<and> test_tools M2 M1 FAIL PM V \<Omega>"
+           (m :: nat) . 
+              OFSM M1 \<and> OFSM M2 \<and> asc_fault_domain M2 M1 m \<and> test_tools M2 M1 FAIL PM V \<Omega>"
 proof 
   show "\<exists>(M1::(nat,nat,nat) FSM)
          (FAIL::(nat\<times>nat))
          (PM::(nat,nat,nat\<times>nat) FSM)
          (V::(nat list set)) 
          (\<Omega>::(nat,nat) ATC set)
-         (m :: nat) . OFSM M1 \<and> OFSM M\<^sub>S \<and> asc_fault_domain M\<^sub>S M1 m \<and> test_tools M\<^sub>S M1 FAIL PM V \<Omega>"
+         (m :: nat) . 
+            OFSM M1 \<and> OFSM M\<^sub>S \<and> asc_fault_domain M\<^sub>S M1 m \<and> test_tools M\<^sub>S M1 FAIL PM V \<Omega>"
   
   proof
     show "\<exists>(FAIL::(nat\<times>nat))
            (PM::(nat,nat,nat\<times>nat) FSM)
            (V::(nat list set)) 
            (\<Omega>::(nat,nat) ATC set)
-           (m :: nat) . OFSM M\<^sub>I \<and> OFSM M\<^sub>S \<and> asc_fault_domain M\<^sub>S M\<^sub>I m \<and> test_tools M\<^sub>S M\<^sub>I FAIL PM V \<Omega>"
+           (m :: nat) . 
+              OFSM M\<^sub>I \<and> OFSM M\<^sub>S \<and> asc_fault_domain M\<^sub>S M\<^sub>I m \<and> test_tools M\<^sub>S M\<^sub>I FAIL PM V \<Omega>"
     proof 
       show "\<exists>(PM::(nat,nat,nat\<times>nat) FSM)
              (V::(nat list set)) 
              (\<Omega>::(nat,nat) ATC set)
-             (m :: nat) . OFSM M\<^sub>I \<and> OFSM M\<^sub>S \<and> asc_fault_domain M\<^sub>S M\<^sub>I m \<and> test_tools M\<^sub>S M\<^sub>I FAIL\<^sub>I PM V \<Omega>"
+             (m :: nat) . 
+                OFSM M\<^sub>I \<and> OFSM M\<^sub>S \<and> asc_fault_domain M\<^sub>S M\<^sub>I m \<and> test_tools M\<^sub>S M\<^sub>I FAIL\<^sub>I PM V \<Omega>"
       proof
         show "\<exists>(V::(nat list set)) 
                (\<Omega>::(nat,nat) ATC set)
-               (m :: nat) . OFSM M\<^sub>I \<and> OFSM M\<^sub>S \<and> asc_fault_domain M\<^sub>S M\<^sub>I m \<and> test_tools M\<^sub>S M\<^sub>I FAIL\<^sub>I PM\<^sub>I V \<Omega>"
+               (m :: nat) . 
+                  OFSM M\<^sub>I \<and> OFSM M\<^sub>S \<and> asc_fault_domain M\<^sub>S M\<^sub>I m \<and> test_tools M\<^sub>S M\<^sub>I FAIL\<^sub>I PM\<^sub>I V \<Omega>"
         proof
           show "\<exists>(\<Omega>::(nat,nat) ATC set)
-                 (m :: nat) . OFSM M\<^sub>I \<and> OFSM M\<^sub>S \<and> asc_fault_domain M\<^sub>S M\<^sub>I m \<and> test_tools M\<^sub>S M\<^sub>I FAIL\<^sub>I PM\<^sub>I V\<^sub>I \<Omega>"
+                 (m :: nat) . 
+                    OFSM M\<^sub>I \<and> OFSM M\<^sub>S \<and> asc_fault_domain M\<^sub>S M\<^sub>I m \<and> test_tools M\<^sub>S M\<^sub>I FAIL\<^sub>I PM\<^sub>I V\<^sub>I \<Omega>"
           proof 
-            show "\<exists>(m :: nat) . OFSM M\<^sub>I \<and> OFSM M\<^sub>S \<and> asc_fault_domain M\<^sub>S M\<^sub>I m \<and> test_tools M\<^sub>S M\<^sub>I FAIL\<^sub>I PM\<^sub>I V\<^sub>I \<Omega>\<^sub>I"
+            show "\<exists>(m :: nat) . 
+                    OFSM M\<^sub>I \<and> OFSM M\<^sub>S \<and> asc_fault_domain M\<^sub>S M\<^sub>I m \<and> test_tools M\<^sub>S M\<^sub>I FAIL\<^sub>I PM\<^sub>I V\<^sub>I \<Omega>\<^sub>I"
             proof
               show "OFSM M\<^sub>I \<and> OFSM M\<^sub>S \<and> asc_fault_domain M\<^sub>S M\<^sub>I 2 \<and> test_tools M\<^sub>S M\<^sub>I FAIL\<^sub>I PM\<^sub>I V\<^sub>I \<Omega>\<^sub>I"
                 using example_OFSM(2,1) example_fault_domain example_test_tools by linarith
